Proved soundness for division expressions.

ch2o_compcertc_lp64.v
@@ -2,7 +2,9 @@ From ch2o_compcert Require Export ch2o_safety compcertc_safety.
 From ch2o Require Export stringmap types expressions statements architectures state.
 (* We prove soundness for LP64 architectures. *)
 From ch2o_compcert Require Export ch2o_lp64.
-From compcert Require Export Csyntax Ctypes Globalenvs.
+From compcert Require Export Cop Csyntax Ctypes Globalenvs.
+
+From Coq Require Import Classical.
 
 Section Program.
 
@@ -13,7 +15,12 @@ Context (Γ: types.env K) (δ: funenv K) (p: Csyntax.program).
 Inductive expr_equiv: expressions.expr K → Csyntax.expr → Prop :=
 | expr_equiv_val_int z:
   int_typed z (sintT: int_type K) → (* TODO: Require the CH2O program to be well-typed instead? *)
-  expr_equiv (EVal ∅ (inr (intV{sintT} z))) (Eval (Vint (Int.repr z)) (Tint I32 Signed noattr)).
+  expr_equiv (EVal ∅ (inr (intV{sintT} z))) (Eval (Vint (Int.repr z)) (Tint I32 Signed noattr))
+| expr_equiv_div e1 ė1 e2 ė2:
+  expr_equiv e1 ė1 →
+  expr_equiv e2 ė2 →
+  expr_equiv (e1 / e2) (Ebinop Odiv ė1 ė2 (Tint I32 Signed noattr))
+.
 
 Inductive stmt_equiv: stmt K → statement → Prop :=
 | stmt_equiv_Return e ė:
@@ -81,6 +88,628 @@ rewrite -> (List.forallb_forall (A:=AST.ident * AST.globdef (Ctypes.fundef F) ty
 apply H.
 Qed.
 
+Lemma int_typed_limits z:
+  int_typed z (sintT%IT: int_type K) →
+  (Int.min_signed ≤ z ∧ z ≤ Int.max_signed)%Z.
+Proof.
+intros.
+unfold Int.min_signed, Int.max_signed.
+unfold Int.half_modulus.
+unfold Int.modulus.
+unfold Int.wordsize.
+unfold Wordsize_32.wordsize.
+assert ((two_power_nat 32 / 2 = 2147483648)%Z). reflexivity.
+rewrite H0.
+destruct H.
+unfold int_lower in H. unfold int_upper in H1.
+simpl in *.
+lia.
+Qed.
+
+Local Open Scope list_scope.
+
+Lemma destruct_list_snoc{X}(P: list X → Prop)(xs: list X):
+  P [] →
+  (∀ xs0 x, P (xs0 ++ [x])) →
+  P xs.
+Proof.
+intros.
+destruct xs.
+- assumption.
+- destruct (exists_last (l:=x::xs)).
+  + intro; discriminate.
+  + destruct s.
+    rewrite e.
+    apply H0.
+Qed.
+
+Lemma compcertc_expr_never_stuck f a k e m:
+  (∃ v ty, a = Eval v ty) ∨
+  ∃ t s, Step (semantics p) (ExprState f a k e m) t s.
+Proof.
+destruct (classic (imm_safe (globalenv p) e RV a m)).
+- inversion H; clear H; subst.
+  + left.
+    eexists; eexists; reflexivity.
+  + right.
+    eexists; eexists.
+    left.
+    apply step_lred; eassumption.
+  + right.
+    eexists; eexists.
+    left.
+    apply step_rred; eassumption.
+  + right.
+    eexists; eexists.
+    left.
+    apply step_call; eassumption.
+- right.
+  eexists; eexists.
+  left.
+  eapply step_stuck with (C:=λ x, x).
+  + apply ctx_top.
+  + eassumption.
+Qed.
+
+Lemma expr_equiv_no_LV_context e ė:
+  expr_equiv e ė →
+  ∀ C a,
+  context LV RV C →
+  ė ≠ C a.
+Proof.
+induction 1; intros.
+- inversion H0; clear H0; subst; discriminate.
+- intro.
+  inversion H1; clear H1; subst; try discriminate.
+  + injection H2; clear H2; intros; subst.
+    eelim IHexpr_equiv1 with (1:=H3); reflexivity.
+  + injection H2; clear H2; intros; subst.
+    eelim IHexpr_equiv2 with (1:=H3); reflexivity.
+Qed.
+
+Notation tint := (Tint I32 Signed noattr).
+
+Lemma sem_cast_int z m:
+  sem_cast (Vint (Int.repr z)) tint tint m = Some (Vint (Int.repr z)).
+Proof.
+  unfold sem_cast.
+  simpl.
+  destruct Archi.ptr64; reflexivity.
+Qed.
+
+Lemma Int_min_signed: Int.min_signed = (-2147483648)%Z.
+Proof.
+reflexivity.
+Qed.
+
+Lemma Int_max_signed: Int.max_signed = 2147483647%Z.
+Proof.
+reflexivity.
+Qed.
+
+Lemma int_lower_sintT: int_lower (sintT%IT: int_type K) = (-2147483648)%Z.
+Proof.
+reflexivity.
+Qed.
+
+Lemma int_upper_sintT: int_upper (sintT%IT: int_type K) = 2147483648%Z.
+Proof.
+unfold int_upper.
+simpl.
+reflexivity.
+Qed.
+
+Lemma rred_safe e ė:
+  expr_equiv e ė →
+  ∀ C a ẽ ṁ t a' ṁ' ρ m,
+  context RV RV C →
+  ė = C a →
+  rred ẽ a ṁ t a' ṁ' →
+  ∃ (E: ectx K) e1 e2,
+  e = subst E e1 ∧
+  Γ \ ρ ⊢ₕ e1, m ⇒ e2, m ∧
+  expr_equiv (subst E e2) (C a') ∧
+  ṁ' = ṁ.
+Proof.
+induction 1; intros.
+- inversion H0; clear H0; subst; try discriminate.
+  subst.
+  inversion H2.
+- inversion H1; clear H1; subst; try discriminate.
+  + subst.
+    inversion H3; clear H3; subst.
+    inversion H; clear H; subst.
+    inversion H0; clear H0; subst.
+    simpl in H10.
+    unfold sem_div in H10.
+    unfold sem_binarith in H10.
+    simpl in H10.
+    rewrite sem_cast_int in H10.
+    rewrite sem_cast_int in H10.
+    rewrite Int.eq_signed in H10.
+    destruct (Coqlib.zeq (Int.signed (Int.repr z0)) (Int.signed Int.zero)). {
+      discriminate.
+    }
+    rewrite Int.signed_repr in n. 2:{ apply int_typed_limits; assumption. }
+    rewrite Int.signed_zero in n.
+    rewrite Int.eq_signed in H10.
+    rewrite Int.signed_repr in H10. 2:{ apply int_typed_limits; assumption. }
+    rewrite Int.signed_repr in H10. 2:{
+      split; try reflexivity.
+      pose proof Int.min_signed_neg.
+      pose proof Int.max_signed_pos.
+      lia.
+    }
+    rewrite Int.eq_signed in H10.
+    rewrite Int.signed_repr in H10. 2:{ apply int_typed_limits; assumption. }
+    rewrite Int.signed_mone in H10.
+    rewrite Int_min_signed in H10.
+    assert (int_typed (z ÷ z0)%Z (sintT: int_type K) ∧ v = Vint (Int.divs (Int.repr z) (Int.repr z0))). {
+      destruct (Coqlib.zeq z (-2147483648)).
+      - destruct (Coqlib.zeq z0 (-1)). {
+          discriminate.
+        }
+        simpl in H10.
+        split; try congruence.
+        subst.
+        split.
+        + rewrite int_lower_sintT.
+          destruct (Z.lt_total z0 0) as [?|[?|?]].
+          * assert (0 <= 2147483648 ÷ -z0)%Z. apply Z.quot_pos; lia.
+            rewrite Zquot.Zquot_opp_r in H0.
+            rewrite <- Zquot.Zquot_opp_l in H0.
+            assert (-(2147483648) = -2147483648)%Z. reflexivity.
+            rewrite H1 in H0.
+            lia.
+          * lia.
+          * destruct (Zquot.Z_mult_quot_ge (-2147483648) z0)%Z; try lia.
+            lapply (Z.mul_le_mono_nonpos_r 1 z0 (-2147483648 ÷ z0))%Z. 2:{
+              assert (-2147483648 ÷ z0 = -(2147483648 ÷ z0))%Z. {
+                rewrite <- Zquot.Zquot_opp_l.
+                reflexivity.
+              }
+              rewrite H4.
+              lapply (Zquot.Z_quot_pos 2147483648 z0). 2:{
+                lia.
+              }
+              intro.
+              lapply H5. 2:{
+                lia.
+              }
+              intro.
+              lia.
+            }
+            intro.
+            lapply H4. 2:{
+              lia.
+            }
+            intro.
+            lia.
+        + rewrite int_upper_sintT.
+          destruct (Z.lt_total 0 z0) as [?|[?|?]].
+          * assert (-2147483648 ÷ z0 = -(2147483648 ÷ z0))%Z. {
+              rewrite <- Zquot.Zquot_opp_l.
+              reflexivity.
+            }
+            rewrite H0.
+            lapply (Zquot.Z_quot_pos 2147483648 z0)%Z; intros. 2:{
+              lia.
+            }
+            lapply H1; intros. 2:{ lia. }
+            lia.
+          * lia.
+          * assert (2147483648 ÷ -z0 < 2147483648)%Z. {
+              apply Z.quot_lt; lia.
+            }
+            rewrite Zquot.Zquot_opp_r in H0.
+            rewrite <- Zquot.Zquot_opp_l in H0.
+            apply H0.
+      - simpl in H10.
+        split; try congruence.
+        split.
+        + rewrite int_lower_sintT.
+          destruct (Z.lt_total 0 z0) as [?|[?|?]]; try lia.
+          * destruct (Z.lt_total 0 z) as [?|[?|?]].
+            -- assert (0 <= z ÷ z0)%Z. apply Zquot.Z_quot_pos; lia.
+               lia.
+            -- subst.
+               rewrite Zquot.Zquot_0_l.
+               lia.
+            -- destruct H3.
+               rewrite int_lower_sintT in H1.
+               assert (z <= z0 * (z ÷ z0))%Z. apply Zquot.Z_mult_quot_ge. lia.
+               assert (z0 * (z ÷ z0) <= 1 * (z ÷ z0))%Z. {
+                 apply Z.mul_le_mono_nonpos_r.
+                 - assert (0 <= -z ÷ z0)%Z. apply Zquot.Z_quot_pos; lia.
+                   assert (-z ÷ z0 = -(z ÷ z0))%Z. rewrite Zquot.Zquot_opp_l; reflexivity.
+                   lia.
+                 - lia.
+               }
+               lia.
+          * destruct (Z.lt_total 0 z) as [?|[?|?]].
+            -- destruct H3.
+               rewrite int_upper_sintT in H3.
+               assert (-z <= -z0 * (-z ÷ -z0))%Z. apply Zquot.Z_mult_quot_ge. lia.
+               assert (-z0 * (-z ÷ -z0) <= 1 * (-z ÷ -z0))%Z. {
+                 apply Z.mul_le_mono_nonpos_r.
+                 - assert (0 <= z ÷ -z0)%Z. apply Zquot.Z_quot_pos; lia.
+                   assert (-z ÷ -z0 = -(z ÷ -z0))%Z. rewrite Zquot.Zquot_opp_l; reflexivity.
+                   lia.
+                 - lia.
+               }
+               assert (-z ÷ -z0 = z ÷ z0)%Z. rewrite Zquot.Zquot_opp_l. rewrite Zquot.Zquot_opp_r. lia.
+               lia.
+            -- subst.
+               rewrite Zquot.Zquot_0_l.
+               lia.
+            -- assert (0 <= z ÷ z0)%Z. {
+                 assert (z ÷ z0 = - -(-z ÷ -z0))%Z. rewrite Zquot.Zquot_opp_l. rewrite Zquot.Zquot_opp_r. lia.
+                 assert (0 <= -z ÷ -z0)%Z. apply Zquot.Z_quot_pos; lia.
+                 lia.
+               }
+               lia.
+        + rewrite int_upper_sintT.
+          destruct (Z.lt_total 0 z0) as [?|[?|?]]; try lia.
+          * destruct (Z.lt_total 0 z) as [?|[?|]].
+            -- destruct H3.
+               rewrite int_upper_sintT in H3.
+               assert (z0 * (z ÷ z0) <= z)%Z. {
+                 apply Zquot.Z_mult_quot_le; lia.
+               }
+               assert (1 * (z ÷ z0) <= z0 * (z ÷ z0))%Z. {
+                 apply Z.mul_le_mono_nonneg_r.
+                 - apply Zquot.Z_quot_pos; lia.
+                 - lia.
+               }
+               lia.
+            -- subst.
+               rewrite Zquot.Zquot_0_l.
+               lia.
+            -- assert (z ÷ z0 = -(-z ÷ z0))%Z. rewrite Zquot.Zquot_opp_l; lia.
+               assert (0 <= -z ÷ z0)%Z. apply Zquot.Z_quot_pos; lia.
+               lia.
+          * destruct (Z.lt_total 0 z) as [?|[?|?]].
+            -- assert (z ÷ z0 = -(z ÷ -z0))%Z. rewrite Zquot.Zquot_opp_r; lia.
+               assert (0 <= z ÷ -z0)%Z. apply Zquot.Z_quot_pos; lia.
+               lia.
+            -- subst.
+               rewrite Zquot.Zquot_0_l.
+               lia.
+            -- destruct H3.
+               rewrite int_lower_sintT in H1.
+               assert (-z0 * (-z ÷ -z0) <= -z)%Z. {
+                 apply Zquot.Z_mult_quot_le; lia.
+               }
+               assert (1 * (-z ÷ -z0) <= -z0 * (-z ÷ -z0))%Z. {
+                 apply Z.mul_le_mono_nonneg_r.
+                 - apply Zquot.Z_quot_pos; lia.
+                 - lia.
+               }
+               assert (z ÷ z0 = -z ÷ -z0)%Z. {
+                 rewrite Zquot.Zquot_opp_l.
+                 rewrite Zquot.Zquot_opp_r.
+                 lia.
+               }
+               lia.
+    }
+    destruct H.
+    subst.
+    exists [].
+    eexists; eexists.
+    simpl; split; [reflexivity|].
+    split. {
+      constructor. constructor.
+      -- assumption.
+      -- apply H.
+    }
+    split. {
+      rewrite (right_id_L _ (∪)).
+      unfold Int.divs.
+      rewrite Int.signed_repr. 2:{ apply int_typed_limits; assumption. }
+      rewrite Int.signed_repr. 2:{ apply int_typed_limits; assumption. }
+      constructor.
+      assumption.
+    }
+    reflexivity.
+  + injection H2; clear H2; intros; subst.
+    destruct (IHexpr_equiv1 C0 a ẽ ṁ t a' ṁ' ρ m H4) as [E [e5 [e6 [? [? ?]]]]]; try trivial.
+    exists (E ++ [CBinOpL (ArithOp DivOp) e2])%E; eexists; eexists.
+    rewrite subst_snoc.
+    rewrite subst_snoc.
+    simpl.
+    rewrite H1.
+    split; try trivial.
+    split. { apply H2. }
+    split. { constructor; tauto. }
+    destruct H5; congruence.
+  + injection H2; clear H2; intros; subst.
+    destruct (IHexpr_equiv2 C0 a ẽ ṁ t a' ṁ' ρ m H4) as [E [e5 [e6 [? [? [? Hṁ']]]]]]; try trivial.
+    exists (E ++ [CBinOpR (ArithOp DivOp) e1])%E; eexists; eexists.
+    rewrite subst_snoc.
+    rewrite subst_snoc.
+    simpl.
+    rewrite H1.
+    split; try trivial.
+    split. { apply H2. }
+    split. { constructor; assumption. }
+    assumption.
+Qed.
+
+Lemma expr_equiv_no_call e ė:
+  expr_equiv e ė →
+  ∀ a m fd vargs ty C,
+  callred (globalenv p) a m fd vargs ty →
+  context RV RV C →
+  ė ≠ C a.
+Proof.
+induction 1; intros.
+- inversion H1; subst; try discriminate.
+  intro; subst.
+  inversion H0.
+- inversion H2; subst; try discriminate.
+  + intro; subst.
+    inversion H1.
+  + intro.
+    injection H4; clear H4; intros; subst.
+    apply IHexpr_equiv1 with (1:=H1) (2:=H3) (3:=eq_refl).
+  + intro.
+    injection H4; clear H4; intros; subst.
+    apply IHexpr_equiv2 with (1:=H1) (2:=H3) (3:=eq_refl).
+Qed.
+
+Lemma expr_equiv_imm_safe_rred e ė:
+  expr_equiv e ė →
+  ∀ ρ m,
+  (∀ (E: ectx K) e1, e = subst E e1 → is_redex e1 → Γ \ ρ ⊢ₕ safe e1, m) →
+  (∃ v ty, ė = Eval v ty) ∨
+  ∀ ṁ,
+  ∃ C a t a',
+  context RV RV C ∧
+  ė = C a ∧ rred (globalenv p) a ṁ t a' ṁ.
+Proof.
+induction 1; intros.
+- left. eexists; eexists; reflexivity.
+- right.
+  intros.
+  destruct (IHexpr_equiv1 ρ m). {
+    intros.
+    apply H1 with (2:=H3) (E:=(E++[CBinOpL (ArithOp DivOp) e2])).
+    rewrite subst_snoc.
+    rewrite H2.
+    reflexivity.
+  }
+  + destruct (IHexpr_equiv2 ρ m). {
+      intros.
+      apply H1 with (2:=H4) (E:=(E++[CBinOpR (ArithOp DivOp) e1])).
+      rewrite subst_snoc.
+      rewrite H3.
+      reflexivity.
+    }
+    * destruct H2 as [v1 [ty1 ?]].
+      destruct H3 as [v2 [ty2 ?]].
+      subst.
+      inversion H; clear H; subst.
+      inversion H0; clear H0; subst.
+      eexists; eexists; eexists; eexists.
+      split. { apply ctx_top. }
+      split. { simpl; reflexivity. }
+      constructor.
+      simpl.
+      assert (Γ \ ρ ⊢ₕ safe (# intV{sintT} z / # intV{sintT} z0)%E, m). {
+        apply H1 with (E:=[]).
+        - reflexivity.
+        - constructor; constructor.
+      }
+      inversion H; clear H; subst.
+      inversion H0; clear H0; subst.
+      inversion H11; clear H11; subst.
+      assert (z0 ≠ 0)%Z. { apply H. }
+      assert (int_typed (z ÷ z0) (sintT%IT: int_type K)). { apply H0. }
+      clear H H0.
+      unfold sem_div.
+      unfold sem_binarith.
+      simpl.
+      rewrite sem_cast_int.
+      rewrite sem_cast_int.
+      rewrite Int.eq_signed.
+      rewrite Int.signed_repr. 2:{ apply int_typed_limits; assumption. }
+      rewrite Int.signed_zero.
+      destruct (Coqlib.zeq z0 0); try lia.
+      simpl.
+      rewrite Int.eq_signed.
+      rewrite Int.signed_repr. 2:{ apply int_typed_limits; assumption. }
+      rewrite Int.signed_repr. 2:{
+        split. { reflexivity. }
+        pose proof Int.min_signed_neg.
+        pose proof Int.max_signed_pos.
+        lia.
+      }
+      rewrite Int_min_signed.
+      rewrite Int.eq_signed.
+      rewrite Int.signed_repr. 2:{ apply int_typed_limits; assumption. }
+      rewrite Int.signed_mone.
+      assert (
+        (if Coqlib.zeq z (-2147483648) then true else false) &&
+        (if Coqlib.zeq z0 (-1) then true else false)
+        = false
+      ). {
+        destruct (Coqlib.zeq z (-2147483648)). {
+          destruct (Coqlib.zeq z0 (-1)). {
+            subst.
+            destruct H5.
+            rewrite int_upper_sintT in H0.
+            discriminate.
+          }
+          reflexivity.
+        }
+        reflexivity.
+      }
+      rewrite H.
+      reflexivity.
+    * destruct (H3 ṁ) as [C [a [t [a' [HC [Hė2 Hrred]]]]]].
+      subst.
+      exists (λ x, Ebinop Odiv ė1 (C x) tint).
+      eexists; eexists; eexists.
+      split. {
+        constructor.
+        assumption.
+      }
+      split. {
+        reflexivity.
+      }
+      eapply Hrred.
+  + destruct (H2 ṁ) as [C [a [t [a' [HC [Hė1 Hrred]]]]]].
+    subst.
+    exists (λ x, Ebinop Odiv (C x) ė2 tint).
+    eexists; eexists; eexists.
+    split. {
+      constructor.
+      assumption.
+    }
+    split. {
+      reflexivity.
+    }
+    eapply Hrred.
+Qed.
+
+Lemma expr_equiv_imm_safe e ė:
+  expr_equiv e ė →
+  ∀ K_ C a ρ m ẽ ṁ,
+  context K_ RV C →
+  ė = C a →
+  (∀ (E: ectx K) e1, e = subst E e1 → is_redex e1 → Γ \ ρ ⊢ₕ safe e1, m) →
+  imm_safe (globalenv p) ẽ K_ a ṁ.
+Proof.
+induction 1; intros.
+- inversion H0; clear H0; subst; try discriminate.
+  subst.
+  constructor.
+- inversion H1; clear H1; subst; try discriminate.
+  + subst.
+    edestruct (expr_equiv_imm_safe_rred (e1 / e2) (Ebinop Odiv ė1 ė2 tint))%E. {
+      constructor; assumption.
+    } {
+      eassumption.
+    }
+    * destruct H1 as [? [? ?]]; discriminate.
+    * destruct (H1 ṁ) as [C [a [t [a' [HC [Hė Hrred]]]]]].
+      rewrite Hė.
+      eapply imm_safe_rred with (C:=C) (e0:=a); eassumption.
+  + injection H2; clear H2; intros; subst.
+    eapply IHexpr_equiv1; try eassumption.
+    * reflexivity.
+    * intros.
+      eapply H3 with (E:=E++[CBinOpL (ArithOp DivOp) e2]); try assumption.
+      rewrite subst_snoc.
+      simpl.
+      congruence.
+  + injection H2; clear H2; intros; subst.
+    eapply IHexpr_equiv2; try eassumption.
+    * reflexivity.
+    * intros.
+      eapply H3 with (E:=E++[CBinOpR (ArithOp DivOp) e1]); try assumption.
+      rewrite subst_snoc.
+      simpl.
+      congruence.
+Qed.
+
+Lemma eval_soundness Q n e ė k ḳ m ṁ f:
+  expr_equiv e ė →
+  ch2o_safe_state Γ δ Q (State k (Expr (cast{sintT%T} e)) m) →
+  (∀ z n',
+   n' ≤ n →
+   int_typed z (sintT: int_type K) →
+   ch2o_safe_state Γ δ Q (State k (Expr (# intV{sintT} z)) m) →
+   compcertc_safe_state_n Q p n' (ExprState f (Eval (Vint (Int.repr z)) (Tint I32 Signed noattr)) ḳ empty_env ṁ)) →
+  compcertc_safe_state_n Q p n (ExprState f ė ḳ empty_env ṁ).
+Proof.
+revert e ė.
+apply well_founded_induction with (1:=lt_wf) (a:=n).
+clear n.
+intros n IH.
+intros.
+intros t s HstarN.
+inversion HstarN; subst.
+- (* refl *)
+  destruct (compcertc_expr_never_stuck f ė ḳ empty_env ṁ).
+  + destruct H2 as [v [ty H2]].
+    subst.
+    inversion H; clear H; subst.
+    unfold compcertc_safe_state_n in H1.
+    eapply H1 with (n':=0) (trace:=[]); try eauto.
+    intro; intros; eapply H0.
+    eapply rtc_l; try eassumption.
+    apply cstep_expr_head with (E:=[]).
+    constructor.
+    apply H4.
+  + tauto.
+- case_eq (match ė with Eval _ _ => true | _ => false end); intros. {
+    inversion H; clear H; subst; try discriminate.
+    unfold compcertc_safe_state_n in H1.
+    eapply H1 with (n':=S n0) (4:=HstarN); try eauto.
+    intro; intros; eapply H0.
+    eapply rtc_l; try eassumption.
+    apply cstep_expr_head with (E:=[]).
+    constructor.
+    apply H5.
+  }
+  destruct H2. 2:{
+    inversion H2; subst; discriminate.
+  }
+  inversion H2; clear H2; subst.
+  + (* step_lred *)
+    eapply expr_equiv_no_LV_context in H; [elim H; reflexivity | assumption].
+  + (* step_rred *)
+    edestruct (rred_safe _ _ H) as [E [e1 [e2 [He1 [He1e2 [Hee' Hṁ']]]]]]; try (eassumption || reflexivity).
+    unfold compcertc_safe_state_n in IH.
+    subst.
+    eapply IH with (2:=Hee') (5:=H3).
+    * lia.
+    * intro S'.
+      intro HS'.
+      apply H0.
+      eapply rtc_l; try eassumption.
+      assert (∀ e, cast{sintT%T} (subst E e) = subst (E ++ [CCast (sintT%T)]) e)%E. {
+        intros; rewrite subst_snoc.
+        reflexivity.
+      }
+      rewrite 2 H2.
+      apply cstep_expr_head.
+      apply He1e2.
+    * intros z n' Hn'.
+      apply (H1 z n'); lia.
+  + (* step_call *)
+    apply expr_equiv_no_call with (2:=H12) (3:=H13) in H.
+    elim H; reflexivity.
+  + elim H13.
+    eapply expr_equiv_imm_safe with (1:=H) (2:=H12). { reflexivity. }
+    intros.
+    destruct (classic (Γ \ locals k ⊢ₕ safe e1, m)); try eassumption.
+    destruct (H0 (State k (Undef (UndefExpr (E ++ [CCast sintT]) e1)) m)). {
+      eapply rtc_l; [|apply rtc_refl].
+      subst.
+      assert (cast{sintT%T} (subst E e1) = subst (E ++ [CCast sintT]) e1)%E. rewrite subst_snoc; reflexivity.
+      rewrite H2.
+      apply cstep_expr_undef; assumption.
+    }
+    * inversion H7.
+    * destruct H7 as [S'' H7].
+      inversion H7.
+Qed.
+
+(*
+
+Inductive state_equiv: state K → Csem.state → Prop :=
+| state_equiv_expr e ė e0 f m:
+  expr_equiv e ė →
+  state_equiv
+    (State [CExpr (cast{sintT%T} e0) (ret □); CParams "main" []] (Expr e) ∅)
+    (ExprState f ė
+       (Kreturn (Kseq (Sreturn (Some (Eval (Vint (Int.repr 0)) (Tint I32 Signed noattr)))) Kstop))
+       empty_env
+       m)
+*)
+
 Theorem soundness Q:
   program_equiv →
   ch2o_safe_program Γ δ Q →
@@ -90,7 +719,7 @@ intros Hequiv Hch2o.
 destruct Hequiv.
 case_eq (Genv.init_mem p); intros; try tauto. clear H0; rename H4 into H0.
 econstructor. { econstructor; try eassumption. reflexivity. }
-intro; intros.
+intro n; intro; intros.
 (* Callstate *)
 inversion H4; clear H4; subst. {
   right.
@@ -130,8 +759,28 @@ inversion H6; clear H6; subst. {
 }
 inversion H2; clear H2; subst; inversion H4; clear H4; subst.
 (* Returning *)
-inversion H1; clear H1; subst.
-inversion H3; clear H3; subst. {
+eapply eval_soundness; try eassumption. {
+  intro; intros.
+  destruct (Hch2o S'); try tauto.
+  apply rtc_transitive with (2:=H2).
+  (* Showing a CH2O execution *)
+  (* Calling main *)
+  eapply rtc_l. {
+    econstructor.
+    - apply H.
+    - constructor.
+    - reflexivity.
+  }
+  simpl.
+  (* Starting executing ret *)
+  eapply rtc_l. {
+    apply cstep_expr with (E:=CReturnE: statements.esctx_item K) (e0:=(cast{sintT%T} e: expressions.expr K)%E).
+  }
+  constructor.
+}
+intros.
+intro; intros.
+inversion H6; clear H6; subst. {
   right.
   eexists.
   eexists.
@@ -140,70 +789,28 @@ inversion H3; clear H3; subst. {
   - reflexivity.
   - reflexivity.
 }
-inversion H1; clear H1; subst; inversion H3; clear H3; subst; try (inversion H12; clear H12; subst; try discriminate).
-{ subst; inversion H11. }
-{ subst; inversion H11. }
-{ inversion H11; clear H11; subst; try discriminate.
+inversion H7; clear H7; subst; inversion H6; clear H6; subst; try (inversion H16; clear H16; subst; try discriminate).
+{ subst; inversion H15. }
+{ subst; inversion H15. }
+{ inversion H15; clear H15; subst; try discriminate.
   subst.
-  elim H12.
+  elim H16.
   constructor. }
 (* Final state *)
-assert (Cop.sem_cast (Vint (Int.repr z)) (Tint I32 Signed noattr) type_int32s m2 = Some (Vint (Int.repr z))). {
-  unfold Cop.sem_cast in H4.
-  simpl in H4.
-  destruct Archi.ptr64; reflexivity. (* TODO: We may at some point need to make an assumption about this. *)
-}
-rewrite H1 in H4.
-simpl in H4.
-inversion H4; clear H4; subst. 2:{
-  inversion H3; clear H3; subst; inversion H4.
+rewrite sem_cast_int in H8.
+inversion H8; clear H8; subst. 2:{
+  inversion H6; clear H6; subst; inversion H8.
 }
 left.
 constructor.
-rewrite Int.signed_repr. 2:{
-  inversion H2.
-  unfold int_lower in H3; simpl in H3.
-  unfold int_upper in H4; simpl in H4.
-  unfold Int.min_signed; unfold Int.max_signed.
-  unfold Int.half_modulus.
-  unfold Int.modulus.
-  unfold Int.wordsize.
-  unfold Wordsize_32.wordsize.
-  split.
-  - apply H3.
-  - simpl. lia.
-}
+rewrite Int.signed_repr. 2:{ apply int_typed_limits; assumption. }
 (* Proving Q z *)
-destruct (Hch2o (state.State [] (Return "main" (intV{sintT} z)) ∅)). 2:{
-  inversion H3; assumption.
+destruct (H5 (state.State [] (Return "main" (intV{sintT} z)) ∅)). 2:{
+  inversion H6; assumption.
 } 2:{
-  destruct H3.
-  inversion H3.
+  destruct H6.
+  inversion H6.
 }
-(* Showing a CH2O execution *)
-(* Calling main *)
-eapply rtc_l. {
-  econstructor.
-  - apply H.
-  - constructor.
-  - reflexivity.
-}
-simpl.
-(* Starting executing ret *)
-eapply rtc_l. {
-  apply cstep_expr with (E:=CReturnE: statements.esctx_item K) (e:=(cast{sintT%T} (# intV{sintT} z): expressions.expr K)%E).
-}
-(* Evaluating the cast *)
-eapply rtc_l. {
-  apply cstep_expr_head with (E:=[]).
-  constructor.
-  destruct H2. constructor; assumption.
-}
-simpl.
-unfold int_cast.
-unfold arch_int_env.
-unfold int_pre_cast.
-simpl.
 (* Finishing executing ret *)
 eapply rtc_l. {
   constructor.
