compcertc_safety.v
@@ -5,11 +5,14 @@ Inductive compcertc_final_state(Q: Z → Prop): state → Prop :=
   compcertc_final_state_intro i m:
   Q (Int.signed i) → compcertc_final_state Q (Returnstate (Vint i) Kstop m).
 
-Definition compcertc_safe_state(Q: Z → Prop)(p: program)(s: state): Prop :=
-  ∀ n trace s',
+Definition compcertc_safe_state_n(Q: Z → Prop)(p: program)(n: nat)(s: state): Prop :=
+  ∀ trace s',
   starN (Smallstep.step (Csem.semantics p)) (Smallstep.globalenv (Csem.semantics p)) n s trace s' →
   compcertc_final_state Q s' ∨
   ∃ trace' s'', Step (Csem.semantics p) s' trace' s''.
+
+Definition compcertc_safe_state(Q: Z → Prop)(p: program)(s: state): Prop :=
+  ∀ n, compcertc_safe_state_n Q p n s.
 
 Inductive compcertc_safe_program(Q: Z → Prop)(p: program): Prop :=
   compcertc_safe_program_intro s0:
