return_divs_ch2o.v
@@ -1,0 +1,17 @@
+Require Export String.
+Require Export ch2o.abstract_c.frontend.
+
+Local Open Scope string_scope.
+
+Definition decls: list (string * decl) :=
+  [("main",
+    FunDecl [] (CTFun [] (CTInt (CIntType None CIntRank)))
+      (CSReturn
+        (Some
+          (CEBinOp (ArithOp DivOp)
+            (CEBinOp (ArithOp DivOp)
+              (CEConst (CIntType (Some Signed) CIntRank) 17)
+              (CEConst (CIntType (Some Signed) CIntRank) 2))
+            (CEBinOp (ArithOp DivOp)
+              (CEConst (CIntType (Some Signed) CIntRank) 15)
+              (CEConst (CIntType (Some Signed) CIntRank) 5))))))].
